Move HKDF to a separate spec; cleanup a bunch of things, including usage of supported_alg

providers/evercrypt/EverCrypt.HKDF.fsti
@@ -4,108 +4,8 @@ open FStar.Integers
 open EverCrypt.Helpers
 open EverCrypt.Hash
 
-noextract
-unfold let bytes = Spec.Hash.Definitions.bytes
-noextract
-unfold let lbytes = EverCrypt.HMAC.lbytes
-
-/// FUNCTIONAL SPECIFICATION:
-///
-/// * extraction is just HMAC using the salt as key and the input
-///   keying materials as text.
-///
-/// * expansion does its own formatting of input key materials.
-
-open FStar.Seq
-
-let extract a salt ikm = EverCrypt.HMAC.hmac a salt ikm
-
-// [a, prk, info] are fixed.
-// [required] is the number of bytes to be extracted
-// [count] is the number of extracted blocks so far
-// [last] is empty for count=0 then set to the prior tag for chaining.
-let rec expand0 :
-  a: Hash.alg ->
-  prk: bytes ->
-  info: bytes ->
-  required: nat ->
-  count: nat ->
-  last: bytes {
-    let chainLength = if count = 0 then 0 else tagLength a in
-    HMAC.keysized a (Seq.length prk) /\
-    Seq.length last = chainLength /\
-    tagLength a + length info + 1 + blockLength a < maxLength a /\
-    count < 255 /\
-    required <= (255 - count) * tagLength a } ->
-  GTot (lbytes required)
-=
-  fun a prk info required count last ->
-  let count = count + 1 in
-  let text = last @| info @| Seq.create 1 (UInt8.uint_to_t count) in
-  let tag = EverCrypt.HMAC.hmac a prk text in
-  if required <= tagLength a
-  then fst (split tag required)
-  else tag @| expand0 a prk info (required - tagLength a) count tag
-
-let expand:
-  a: Hash.alg ->
-  prk: bytes ->
-  info: bytes ->
-  required: nat {
-    HMAC.keysized a (Seq.length prk) /\
-    tagLength a + length info + 1 + blockLength a < maxLength a /\
-    required <= 255 * tagLength a } ->
-  GTot (lbytes required)
-=
-  fun a prk info required ->
-  expand0 a prk info required 0 Seq.empty
-
-
-(* 18-03-05 TBC, requires TLS libraries
-
-/// Details specific to TLS 1.3; should move to its own module.
-///
-/// Since derivations depend on the concrete info,
-/// we will need to prove format injective.
-
-let tls13_prefix: Bytes.lbytes 6 =
-  let s = Bytes.bytes_of_string "tls_13 " in
-  assume(Bytes.length s = 6); // a bit lame; not sure how to deal with such constants
-  s
-
-let format: (
-  a: Hash.alg ->
-  label: string{length (Bytes.bytes_of_string label) < 256 - 6} ->
-  hv: uint8_p {length hv < 256} ->
-  len: UInt32.t {v len <= 255 * tagLength ha} ->
-  Tot bytes )
-=
-  fun ha label hv len ->
-  let label_bytes = tls13_prefix @| Bytes.reveal (Bytes.bytes_of_string label) in
-  // lemma_repr_bytes_values (v len);
-  // lemma_repr_bytes_values (length label_bytes);
-  // lemma_repr_bytes_values (length hv);
-  FStar.Bytes.(reveal (bytes_of_int 2 (v len) @| vlbytes 1 label_bytes @| vlbytes 1 hv))
-
-val expand_label:
-  #a: Hashing.alg ->
-  prk: hkey a ->
-  label: string{length (bytes_of_string label) < 256 - 6} -> // -9?
-  hv: bytes{length hv < 256} ->
-  length: nat {length <= 255 * tagLength a} -> luint8_p length
-let expand_label #a prk label hv length =
-  expand prk (format a label hv length) length
-
-let expand_secret #a prk label hv = expand_label prk label hv (tagLength a)
-
-/// Details specific to QUIC; could move to its own module
-
-//18-04-10 TODO code in Low* [quic_provider.quic_crypto_hkdf_quic_label]
-
-*)
-
-
-
+open Spec.HKDF
+open Spec.Hash.Definitions
 
 /// IMPLEMENTATION
 
@@ -118,9 +18,9 @@ open LowStar.Buffer
 (** @type: true
 *)
 val hkdf_extract :
-  a       : alg ->
+  a       : EverCrypt.HMAC.supported_alg ->
   prk     : uint8_pl (tagLength a) ->
-  salt    : uint8_p { disjoint salt prk /\ HMAC.keysized a (length salt)} ->
+  salt    : uint8_p { disjoint salt prk /\ Spec.HMAC.keysized a (length salt)} ->
   saltlen : uint8_l salt ->
   ikm     : uint8_p { length ikm + blockLength a < pow2 32 /\ disjoint ikm prk } ->
   ikmlen  : uint8_l ikm -> Stack unit
@@ -129,18 +29,18 @@ val hkdf_extract :
   (ensures  (fun h0 r h1 ->
     live h1 prk /\ LowStar.Modifies.(modifies (loc_buffer prk) h0 h1) /\
     length ikm + blockLength a < maxLength a /\
-    as_seq h1 prk == HMAC.hmac a (as_seq h0 salt) (as_seq h0 ikm)))
+    as_seq h1 prk == Spec.HMAC.hmac a (as_seq h0 salt) (as_seq h0 ikm)))
 
 (** @type: true
 *)
 val hkdf_expand :
-  a       : alg ->
+  a       : EverCrypt.HMAC.supported_alg ->
   okm     : uint8_p ->
   prk     : uint8_p -> prklen  : uint8_l prk ->
   info    : uint8_p -> infolen : uint8_l info ->
   len     : uint8_l okm {
     disjoint okm prk /\
-    HMAC.keysized a (v prklen) /\
+    Spec.HMAC.keysized a (v prklen) /\
     tagLength a + v infolen + 1 + blockLength a < pow2 32 /\
     v len <= 255 * tagLength a } ->
   Stack unit
