specs/Spec.HMAC.fsti
@@ -6,17 +6,15 @@ let is_supported_alg = function
   | SHA1 | SHA2_256 | SHA2_384 | SHA2_512 -> true
   | _ -> false
 
-let ha = a:hash_alg { is_supported_alg a }
-
 let lbytes (l:nat) = b:bytes {Seq.length b = l}
 
-let keysized (a:ha) (l:nat) =
+let keysized (a:hash_alg) (l:nat) =
   l < max_input_length a /\
   l + block_length a < pow2 32
 
 (* ghost specification; its algorithmic definition is given in the .fst *)
 val hmac:
-  a: ha -> //18-07-09 can't mix refinements and erasure??
+  a: hash_alg -> //18-07-09 can't mix refinements and erasure??
   key: bytes{ keysized a (Seq.length key) } ->
   data: bytes{ Seq.length data + block_length a < max_input_length a } ->
   Tot (lbytes (hash_length a))
