specs/Spec.HKDF.fst
@@ -1,0 +1,46 @@
+module Spec.HKDF
+
+open FStar.Integers
+open Spec.Hash.Definitions
+
+/// FUNCTIONAL SPECIFICATION:
+///
+/// * extraction is just HMAC using the salt as key and the input
+///   keying materials as text.
+///
+/// * expansion does its own formatting of input key materials.
+
+open FStar.Seq
+
+let extract = Spec.HMAC.hmac 
+
+// [a, prk, info] are fixed.
+// [required] is the number of bytes to be extracted
+// [count] is the number of extracted blocks so far
+// [last] is empty for count=0 then set to the prior tag for chaining.
+let rec expand0 :
+  a: hash_alg ->
+  prk: bytes ->
+  info: bytes ->
+  required: nat ->
+  count: nat ->
+  last: bytes {
+    let chainLength = if count = 0 then 0 else hash_length a in
+    HMAC.keysized a (Seq.length prk) /\
+    Seq.length last = chainLength /\
+    hash_length a + length info + 1 + block_length a < max_input_length a /\
+    count < 255 /\
+    required <= (255 - count) * hash_length a } ->
+  Tot (lbytes required)
+=
+  fun a prk info required count last ->
+  let count = count + 1 in
+  let text = last @| info @| Seq.create 1 (UInt8.uint_to_t count) in
+  let tag = Spec.HMAC.hmac a prk text in
+  if required <= hash_length a
+  then fst (split tag required)
+  else tag @| expand0 a prk info (required - hash_length a) count tag
+
+let expand a prk info required =
+  expand0 a prk info required 0 Seq.empty
+
